\documentclass[12pt]{article}
\usepackage[a4paper, portrait, margin=1cm, bottom=2cm]{geometry}
\usepackage{fontspec}
\usepackage[fleqn]{amsmath}
\usepackage{amssymb}
\usepackage{indentfirst}
\usepackage{graphicx}
\usepackage{framed}

\setmainfont[Ligatures=TeX]{Linux Libertine}
\graphicspath{./graphics/}

\title{АиГ. ДЗ к 2023-06-01. Дифференциальные уравнения. Вариант №14}
\author{Студент группы 2305 Александр Макурин}
\date{29 мая 2023}

\begin{document}
\maketitle
\section{$y'' - 6y' + 13y = e^{2x}(15x - 21), \ y(0) = -6, \ y'(0) = -10$}
\[
    \lambda^2 - 6\lambda + 13 = 0
    \lambda_{1,2} = \dfrac{6 \pm \sqrt{36 - 52}}{2} = 3 \pm 2i
\]
\[
    y_\text{о} = e^{3x}(C_1\cos{2x} + C_2\sin{2x})
\]
\[
    y_\text{ч} = (D_1x + D_0)e^{2x} \\ y_\text{ч}' = (2D_1x + 2D_0 + D_1)e^{2x} \\ y_\text{ч}'' = (4D_1x + 4D_0 + 4D_1)
\]
\[
    4D_1x + 4D_1 + 4D_0 - 12D_1x - 12D_0 - 6D_1 + 13D_1x + 13D_0 = 15x - 21
\]
\[
    5D_1x - 2D_1 + 5D_0 = 15x - 21
\]
\[
    \begin{cases}
        5D_1 = 15 \\
        5D_0 - 2D_1 = -21
    \end{cases}
    \Rightarrow
    \begin{array}{l}
        D_1 = 3 \\
        D_0 = -3
    \end{array}
\]
\[
    y_\text{ч} = (3x - 3)e^{2x}
\]
\[
    y = (C_1\cos{2x}+C_2\sin{2x})e^{3x} + 3(x - 1)e^{2x}
\]
\[
    y' = (3C_1\cos{2x} + 3C_2\sin{2x} - 2C_1\sin{2x} + 2C_2\cos{2x})e^{3x} + 3(2x - 1)e^{2x}
\]
\[
    \begin{cases}
        C_1 - 3 = -6 \\
        3C_1 + 2C_2 - 3 = -10
    \end{cases}
    \Rightarrow
    \begin{array}{l}
        C_1 = -3 \\
        C_2 = 1
    \end{array}
\]
\fbox{Ответ: $y = (-3\cos{2x} + \sin{2x})e^{3x} + 3(x - 1)e^{2x}$}
\section{$y'' - 5y' + 4y = e^{x}(2\cos{2x} - 16\sin{2x}), \ y(0) = -6, \ y'(0) = -13$}
\[
    \lambda^2 - 5\lambda + 4 = 0
\]
\[
    \lambda_{1,2} = 1, 4
\]
\[
    y_\text{о} = C_1e^x + C_2e^{4x}
\]
\[
    y_\text{ч} = (A\cos{2x} + B\sin{2x})e^x
\]
\[
    y_\text{ч}' = (A\cos{2x} + B\sin{2x} - 2A\sin{2x} + 2B\cos{2x})e^x
\]
\[
    y_\text{ч}'' = (-3A\cos{2x} - 3B\sin{2x} - 4A\sin{2x} + 4B\cos{2x})e^x
\]
\[
    \cos{2x}(-3A + 4B - 5A - 10B + 4A) + \sin{2x}(-4A - 3B - 5B + 10A + 4B) = 2\cos{2x} - 16\sin{2x}
\]
\[
    \begin{cases}
        -4A - 6B = 2 \\
        6A - 4B = -16
    \end{cases}
    \Rightarrow
    \begin{cases}
        A = -\dfrac{3}{2}B - \dfrac{1}{2} \\
        -9B - 3 - 4B = -16
    \end{cases}
    \Rightarrow
    \begin{cases}
        A = -2 \\
        B = 1
    \end{cases}
\]
\[
    y_\text{ч} = (-2\cos{2x} + \sin{2x})e^x
\]
\[
    y = C_1e^x + C_2e^{4x} + e^x\sin{2x} - 2e^x\cos{2x}
\]
\[
    y' = C_1e^x + 4C_2e^{4x} + e^x\sin{2x} - 2e^x\cos{2x} + 2e^x\cos{2x} + 4e^x\sin{2x}
\]
\[
    \begin{cases}
        C_1 + C_2 - 2 = -6 \\
        C_1 + 4C_2 = -13
    \end{cases}
    \Rightarrow
    \begin{cases}
        C_1 = -4 - C_2
        3C_2 - 4 = -13
    \end{cases}
    \Rightarrow
    \begin{cases}
        C_1 = -1 \\
        C_2 = -3
    \end{cases}
\]
\fbox{Ответ: $y = -e^x -3e^{4x} + e^x\sin{2x} - 2e^x\cos{2x}$}
\section{\[
      \left\{\begin{array}{rrrr}
          x' & = & 14x & -15y \\
          y' & = & 6x  & - 5y
      \end{array}\right.
      \\
      \begin{array}{l}
          x(0) = 8 \\
          y(0) = 5
      \end{array}
  \]}
\[
    \begin{vmatrix}
        14 - \lambda & -15          \\
        6            & -5 - \lambda
    \end{vmatrix}
    = -70 - 14\lambda + 5\lambda + \lambda^2 + 90
    = \lambda^2 - 9\lambda + 20 = 0
    \Rightarrow
    \lambda_{1,2} = 4, 5
\]
\[
    \begin{pmatrix}
        10 & -15 \\
        6  & -9
    \end{pmatrix}
    \sim
    \begin{pmatrix}
        2 & -3 \\
        0 & 0
    \end{pmatrix}
    \Rightarrow
    e_1 = \begin{pmatrix}3 \\ 2\end{pmatrix}e^{4t}
\]
\[
    \begin{pmatrix}
        9 & -15 \\
        6 & -10
    \end{pmatrix}
    \sim
    \begin{pmatrix}
        3 & -5 \\
        0 & 0
    \end{pmatrix}
    \Rightarrow
    e_2 = \begin{pmatrix}5 \\ 3\end{pmatrix}e^{5t}
\]
\[
    \begin{cases}
        x(t) = 3C_1e^{4t} + 5C_2e^{5t} \\
        y(t) = 2C_1e^{4t} + 3C_2e^{5t}
    \end{cases}
\]
\[
    \begin{pmatrix}8 \\ 5 \end{pmatrix}
    =
    C_1\begin{pmatrix}3 \\ 2\end{pmatrix}
    +
    C_2\begin{pmatrix}5 \\ 3\end{pmatrix}
    \Rightarrow
    C_1 = C_2 = 1
\]
\[
    X = \begin{pmatrix} x\\y \end{pmatrix}
\]
\fbox{Ответ: $X(t) = \begin{pmatrix}3\\2\end{pmatrix}e^{4t} + \begin{pmatrix}5\\3\end{pmatrix}e^{5t}$}
\end{document}